Add generic Ser/Deser and use in uint8.

src/dafny/ssz/IntSeDes.dfy
@@ -63,21 +63,97 @@ module IntSeDes {
 
     //  Uintk serialisation and deserielisation.
 
+    /**
+     * Computes the serialisation of a natural value.
+     *
+     * @param n     The value to serialise.
+     * @param k     The number of bytes for the the result of the serialisation.
+     *
+     * @returns     The `k`-byte big endian serialisation of `n`.
+     *
+     */
+    function method uintSe(n: nat, k: nat) : seq<byte>
+        requires k >= 1
+        requires n < power2(8 * k) 
+        ensures |uintSe(n, k)| == k
+
+        decreases n, k
+    {
+        if ( k == 1 ) then 
+            [n as byte]
+        else 
+            //  ensures pre-cond for recursive call n / 256 < power2(8 * (k - 1))
+            //  implied by n < power2(8) * power2(8 * (k - 1)) (productRulePower2)
+            productRulePower2(8, 8 * (k - 1));
+            [ (n % 256) as byte] + uintSe( n / 256 , k - 1)
+    }
+
+    /**
+     *  Deserialise a sequence of bytes into a natural number.
+     *
+     *  @param  b   A sequence of at least one byte. 
+     *
+     *  @returns     A natural number obtained by interpreting `b` as big endian.
+     */
+    function method uintDes(b : seq<byte>) : nat
+        requires |b| >= 1
+        ensures uintDes(b) < power2(8 * |b|) 
+
+        decreases b
+    {
+        if ( |b| == 1 ) then 
+            b[0] as nat
+        else 
+            //  Inductive proof of the post-condition uses power2(8) == 256 
+            //  and power2(8) * power2(8 * (|b| - 1)) == power2(8 * |b|) 
+            productRulePower2(8, 8 * (|b| - 1) );
+            (b[0] as nat) + 256 * uintDes(b[1..])
+    }
+
+    /**
+     *  Composition of deserialise and serialise is the identiy.
+     *
+     *  @param  n   A natural number
+     *  @param  k   A number of bytes.
+     */
+    lemma {:induction n, k} involution(n : nat, k : nat)
+        requires n < power2(8 * k) 
+        requires k >= 1
+        ensures uintDes(uintSe(n, k)) == n 
+    {
+        if ( k == 1 ) {
+            //  Thanks Dafny
+        } else {
+            //  Ensuring pre-condition os recursive call to uinSe requires 
+            //  power2(8) * power2(8 * (k - 1)) == power2(8 * k) 
+            productRulePower2(8, 8 * (k - 1));
+            calc == {
+                uintDes(uintSe(n, k));
+                ==
+                uintDes([ (n % 256) as byte] + uintSe( n / 256 , k - 1));
+            }
+        }
+    }
+
+    //  Special cases used in Eth2.0 Specs: Uint_k for k in {8, 16, 32, 64, 128, 256}
+    
     /** Uint8. */
     function method uint8ToBytes(n: uint8) : seq<byte> 
+        requires power2(8) == 0x100
         ensures |uint8ToBytes(n)| == 1
     {
-        [n as byte]
+        uintSe(n as nat, 1)
     }
  
-    function method byteToUint8(b: byte) : uint8
+    function method byteToUint8(b: seq<byte>) : uint8
+        requires |b| == 1
     {
-        (b as uint8)
+        uintDes(b) as uint8
     }
 
     /** Encode/decode Uint8 yields Identity. */
     lemma uint8AsBytesInvolutive(n : uint8) 
-        ensures byteToUint8(uint8ToBytes(n)[0]) == n
+        ensures byteToUint8(uint8ToBytes(n)) == n
     {   //  Thanks Dafny
     }
 
